Deploying to gh-pages from @ xubaiw/reservoir-index@d8e561b4ba43e1d20072319a7eee6520d01bb887 🚀

git/ammkrn/JohnDoe/JohnDoe/Federal/CivilProcedure/Rules.lean
@@ -16,16 +16,16 @@ import JohnDoe.Federal.CivilProcedure.Motion
 import JohnDoe.Federal.CivilProcedure.Period
 import JohnDoe.Federal.CivilProcedure.CivilAction
 
-open Std (HashMap AssocList)
-
 set_option autoImplicit false
+
+open Std (HashMap AssocList)
 
 structure Document where
   contents : String
-  dateTime : TaiDateTime
+  timeStamp : TaiDateTime
 deriving Repr
 
-structure Store where
+structure Config where
   documents : List Document
   status : Status
   dateTime : TaiDateTime
@@ -35,89 +35,182 @@ structure Store where
   complaint : FiledComplaint
   removedByDefendant : Bool
   motions : List Motion
-  summonses : Unit
+  summonses : List SummonsOrWaiver
+
+abbrev CivilActionState := Config
 
 structure ComInfo where
+  /- taken at -/
   dateTime : TaiDateTime
+  /- The accompanying document (if it exists) -/
+  document : Option Document
+  /- Additional information -/
   label : String
-  document : Option (String × TaiDateTime)
 
-structure DCom extends ComInfo where
-  -- Must be true before `f` can be executed.
-  pre : Store → Prop
-  f : ∀ (store : Store), pre store → Store
-  -- Must be true after `f` for `EvalR`.
-  post : Store → Prop
+-- Com
+structure Com extends ComInfo where
+  pre : Config → Prop
+  f : ∀ (store : Config), pre store → Config
+  post : Config → Prop
+  preErrorMsg (cfg : Config) (h : ¬pre cfg) : String
+  postErrorMsg (cfg : Config) (hPre : pre cfg) (hPost : ¬post (f cfg hPre)) : String
+  [decidablePre : DecidablePred pre]
+  [decidablePost : DecidablePred post]
+  --postErrorMsg+ : ∀ cfg cfg', (pre cfg) → (cfg' = f cfg) → ¬post cfg' → Error
 
+instance : ∀ (com : Com), DecidablePred (com.pre) := Com.decidablePre 
+instance : ∀ (com : Com), DecidablePred (com.post) := Com.decidablePost
+
+-- Pgm/ProceduralHistory
 inductive BinTree
-| leaf (com : DCom)
+| leaf (com : Com)
 | node (l r : BinTree) 
 
-inductive EvalR : BinTree → Store → Store → Prop
+abbrev ProceduralHistory := BinTree
+
+inductive BinTree.EvalR : BinTree → Config → Config → Prop
 | leaf 
-  (com : DCom)
-  (store store' : Store)
+  (com : Com)
+  (store store' : Config)
   (hPre : com.pre store)
+  (h : com.f store hPre = store')
   (hPost : com.post store') 
-  (h : com.f store hPre = store') : 
+  (hTime : store.dateTime <= store'.dateTime) :
     EvalR (.leaf com) store store'
 | node 
   (l r : BinTree)
-  (store₀ store₁ store₂ : Store)
+  (store₀ store₁ store₂ : Config)
   (hL : EvalR l store₀ store₁)
-  (hR : EvalR r store₁ store₂) 
-  (hTimeMonoL : store₀.dateTime <= store₁.dateTime)
-  (hTImeMonoR : store₁.dateTime <= store₂.dateTime) : 
+  (hR : EvalR r store₁ store₂) :
     EvalR (.node l r) store₀ store₂ 
 
+/-
+Inversion rule for leaves
+-/
+theorem BinTree.EvalR.leaf_inversion (com : Com) (store store' : Config) :
+  EvalR (.leaf com) store store' ↔ (∃ hPre, com.f store hPre = store' ∧ com.post store' ∧ store.dateTime <= store'.dateTime) := by
+  refine Iff.intro ?mp ?mpr
+  case mp =>
+    intro h; 
+    cases h with
+    | leaf _ _ _ a4 a5 a6 a7 =>
+      exact Exists.intro a4 ⟨a5, a6, a7⟩
+  case mpr =>
+    intro h
+    cases h with
+    | intro w p =>
+      exact EvalR.leaf com store store' w p.left p.right.left p.right.right
+
+/-
+Inversion rule for nodes
+-/
+theorem BinTree.EvalR.node_inversion (l r : BinTree) (store store' : Config) :
+  EvalR (.node l r) store store' ↔ (∃ store_x, EvalR l store store_x ∧ EvalR r store_x store') :=  by
+  refine Iff.intro ?mp ?mpr
+  case mp =>
+    intro h
+    cases h with
+    | node a1 a2 a3 store_x a5 a6 a7 =>
+      exact Exists.intro store_x ⟨a6, a7⟩
+  case mpr =>
+    intro h
+    cases h with
+    | intro w p =>
+      exact EvalR.node l r store w store' p.left p.right
+
+
+theorem timeMono (t : BinTree) (s s' : Config) : 
+  t.EvalR s s' → s.dateTime <= s'.dateTime
+| BinTree.EvalR.leaf _ s s' _ _ _ hTime => hTime
+| BinTree.EvalR.node l r s0 s1 s2 hL hR => 
+  le_trans (timeMono l s0 s1 hL) (timeMono r s1 s2 hR)
+
+abbrev ErrString := String
+
+def BinTree.eval : BinTree → EStateM ErrString Config Unit
+| leaf com => do
+  let cfg ← get
+  if hPre : com.pre cfg
+  then 
+    let cfg' := com.f cfg hPre
+    if ¬cfg.dateTime <= cfg'.dateTime 
+    then 
+      throw "time error"
+    else if ¬com.post cfg'
+    then 
+      throw "failedPostError"
+    else
+      set cfg'
+  else
+    throw "failedPrestateError"
+| node l r => do eval l; eval r
+
+
+theorem BinTree.evalsEquivMp (t : BinTree) (cfg cfg' : Config) :
+  t.EvalR cfg cfg' → t.eval.run cfg = EStateM.Result.ok () cfg'
+| EvalR.leaf c s s' hPre h hPost hT => by
+  simp [BinTree.eval, EStateM.run]
+  simp at hT
+  simp [bind, EStateM.bind, get, getThe, MonadStateOf.get, EStateM.get, hPre, h, hPost, hT, set, EStateM.set]
+| EvalR.node l r _ cfgX _ hL hR => by
+  have ihL := evalsEquivMp l cfg cfgX hL
+  have ihR := evalsEquivMp r cfgX cfg' hR
+  simp [EStateM.run] at ihL ihR
+  simp [BinTree.eval, EStateM.run, bind, EStateM.bind, get, getThe, MonadStateOf.get, EStateM.get, ihL, ihR]
+  done
+
+theorem evalsEquivMpr : 
+  ∀ 
+  (t : BinTree)
+  (cfg cfg' : Config), 
+  t.eval.run cfg = EStateM.Result.ok () cfg' → t.EvalR cfg cfg'
+| BinTree.leaf c, cfg, cfg' => by
+  sorry
+| BinTree.node l r, cfg, cfg' => by
+  sorry
+
 @[reducible]
-def BinTree.pre : BinTree → (Store → Prop)
+def BinTree.pre : BinTree → (Config → Prop)
 | leaf com => com.pre
 | node l _ => l.pre
 
 @[reducible]
-def BinTree.post : BinTree → (Store → Prop)
+def BinTree.post : BinTree → (Config → Prop)
 | leaf com => com.post
 | node _ r => r.post
 
 /-
 if `EvalR t s s'`, then the precondition is true of s
 -/
-theorem EvalRPre 
-  (t : BinTree) 
-  (store store' : Store) 
-  (h : EvalR t store store') : t.pre store := by
-  cases h with
-  | leaf c s s' hPre h hpost => 
-    simp [BinTree.pre]
-    exact hPre
-  | node l r s0 s1 s2 h0 h1 => 
-    simp [BinTree.pre]
-    exact EvalRPre l store s1 h0
+theorem BinTree.EvalR_pre (t : BinTree) (store store' : Config) :
+  t.EvalR store store' → t.pre store
+| EvalR.leaf _ s s' hPre _ _ _ => hPre
+| EvalR.node l _ s0 s1 s2 hL _ => EvalR_pre l s0 s1 hL
 
 /-
 If (EvalR t s s'), then t's post-condition is true of s'.
 -/
-theorem EvalRPost 
-  (t : BinTree) 
-  (store store' : Store) 
-  (h : EvalR t store store') : t.post store' := by
-  cases h with
-  | leaf c s s' hpre h hpost => simp [BinTree.post]; assumption
-  | node l r s0 s1 s2 h0 h1 => exact EvalRPost r s1 store' h1
+theorem BinTree.EvalR_post (t : BinTree) (store store' : Config) :
+  t.EvalR store store' → t.post store'
+| EvalR.leaf _ s s' _ _ hpost _ => hpost 
+| EvalR.node _ r s0 s1 s2 _ ih1 => EvalR_post r s1 s2 ih1
 
-theorem evalDeterministic : 
+private theorem BinTree.EvalR_deterministicAux : 
   ∀ (pgm : BinTree) 
-    (store storeA : Store),
-    EvalR pgm store storeA 
-    → (∀ storeB : Store, EvalR pgm store storeB → storeA = storeB) 
-| (.leaf com), s, storeA, EvalR.leaf _ _ _ _ _ f, sB, EvalR.leaf _ _ _ _ _ i => by rw [← f, ← i]
-| (.node l r), s, storeA, EvalR.node _ _ _ s1 _ P Q _ _, storeB, EvalR.node _ _ _ s1' _ T U _ _ =>
-  have ihl := evalDeterministic l s s1 P s1' T
-  evalDeterministic r s1 storeA Q storeB (ihl ▸ U)
+    (store storeA : Config),
+    pgm.EvalR store storeA 
+    → (∀ storeB : Config, pgm.EvalR store storeB → storeA = storeB) 
+| (.leaf com), s, storeA, EvalR.leaf _ _ _ _ f _ _, sB, EvalR.leaf _ _ _ _ i _ _ => by rw [← f, ← i]
+| (.node l r), s, storeA, EvalR.node _ _ _ s1 _ P Q, storeB, EvalR.node _ _ _ s1' _ T U =>
+  have ihl := EvalR_deterministicAux l s s1 P s1' T
+  EvalR_deterministicAux r s1 storeA Q storeB (ihl ▸ U)
+
+theorem BinTree.EvalR_deterministic (pgm : BinTree) (store storeA storeB : Config) :
+  pgm.EvalR store storeA → pgm.EvalR store storeB → storeA = storeB :=
+  fun hA hB => BinTree.EvalR_deterministicAux pgm store storeA hA storeB hB
 
 -- S₀ ⊆ S
-def Complaint.file (complaint : Complaint) : ∀ (filedOn : TaiDateTime) (caseNum : Nat), Store
+def Complaint.file (complaint : Complaint) : ∀ (filedOn : TaiDateTime) (caseNum : Nat), Config
 | filedOn, caseNum =>
   {
     status := .complaintFiled
@@ -133,53 +226,55 @@ def Complaint.file (complaint : Complaint) : ∀ (filedOn : TaiDateTime) (caseNu
     claims := complaint.claims
     removedByDefendant := false
     motions := []
-    summonses := ()
+    summonses := []
     documents := [
       --(Document.mk (contents := complaint.text) (dateTime := filedOn))
     ]
 }
 
-theorem inversionLeaf (com : DCom) (store store' : Store) :
-  EvalR (.leaf com) store store' ↔ (∃ hPre, com.f store hPre = store' ∧ com.post store') := by
-  refine Iff.intro ?mp ?mpr
-  case mp =>
-    intro h; 
-    cases h with
-    | leaf _ _ _ a4 a5 a6 =>
-      exact Exists.intro a4 (And.intro a6 a5)
-  case mpr =>
-    intro h
-    cases h with
-    | intro w p =>
-      exact EvalR.leaf com store store' w p.right p.left
+/-
+I think because of the monotonicity of time,
+but I don't think it will be necessary to extend the rule discussions to `Store2`.
+-/
+@[reducible]
+def validInitialStates : Set Config :=
+    { cfg | ∃ (complaint : Complaint) (filedOn : TaiDateTime) (caseNum : Nat), cfg = complaint.file filedOn caseNum }
 
-theorem inversionNode (l r : BinTree) (store store' : Store) :
-  EvalR (.node l r) store store' ↔ (∃ store_x, EvalR l store store_x ∧ EvalR r store_x store' ∧ store.dateTime <= store_x.dateTime ∧ store_x.dateTime <= store'.dateTime) :=  by
-  refine Iff.intro ?mp ?mpr
-  case mp =>
-    intro h;
-    cases h with
-    | node a1 a2 a3 store_x a5 a6 a7 a8 =>
-      refine Exists.intro store_x ?r
-      refine And.intro a6 ?r0
-      refine And.intro a7 ?r1
-      refine And.intro a8 ?r2
-      assumption
-  case mpr =>
-    intro h
-    cases h with
-    | intro w p =>
-      apply EvalR.node l r store w store'
-      exact p.left
-      exact p.right.left
-      exact p.right.right.left
-      exact p.right.right.right
+@[reducible]
+def Config.isValidInitialConfig : Config → Prop := (. ∈ validInitialStates)
 
-def validInitialStates : Set Store :=
-    { store | ∃ (complaint : Complaint) (filedOn : TaiDateTime) (caseNum : Nat), store = complaint.file filedOn caseNum }
-
-def EvalRBinary : Store → Store → Prop := fun s s' => ∃ (c : BinTree), EvalR c s s'
+def EvalRBinary : Config → Config → Prop := fun s s' => ∃ (c : BinTree), c.EvalR s s'
 
 def RTC : {α : Type _} → (α → α → Prop) → α → α → Prop := sorry
 
-def Store.reachable (s : Store) := ∃ s₀, s₀ ∈ validInitialStates ∧ @RTC Store EvalRBinary s₀ s
+@[reducible]
+def validTriple (c : BinTree) (s s' : Config) := 
+  s ∈ validInitialStates ∧ c.EvalR s s'
+
+@[reducible]
+def Config.reachable (s : Config) := 
+  ∃ s₀, s₀ ∈ validInitialStates ∧ RTC EvalRBinary s₀ s
+
+@[reducible]
+def Config.reachable' (s : Config) := 
+  ∃ (c : BinTree) (s₀ : Config), validTriple c s₀ s
+
+class Compiler (A : Type) where
+  compile : A → Com
+
+class SerializableCompiler (A : Type) (B : Type) extends Compiler A where
+  encode : A → B
+  decode : B → Option A
+  encodeOk : ∀ a, decode (encode a) = some a
+  
+@[reducible]
+def BinTree.mem (c : Com) : BinTree → Prop
+| leaf x => x = c
+| node l r => mem c l ∨ mem c r
+
+instance : Membership Com BinTree where
+  mem c t := BinTree.mem c t
+
+instance {A : Type} [Compiler A] : Membership A BinTree where
+  mem a t := (Compiler.compile a) ∈ t
+
