git/tydeu/lean4-alloy/examples/my_add/MyAdd.lean
@@ -1,0 +1,8 @@
+import Alloy.C
+open scoped Alloy.C
+
+alloy c include <lean/lean.h>
+
+alloy c extern def myAdd (x y : UInt32) : UInt32 := {
+  return x + y;
+}
