git/xubaiw/Dta.lean/Dta/Float.lean
@@ -1,9 +1,0 @@
-namespace Dta
-
-@[extern c inline "(double)(#1)"]
-opaque uint16ToFloat : UInt16 → Float
-
-@[extern c inline "(double)(#1)"]
-opaque uint32ToDouble : UInt32 → Float
-
-end Dta
