git/xubaiw/Dta.lean/Dta/Parser.lean
@@ -1,21 +1,20 @@
 import Dta.Basic
-import Dta.Float
 import Parsec
 
-open Parsec ByteArrayParser
+open Parsec Binary Parser
 
 namespace Dta
 
-def wrapped (tag : String) (p : ByteArrayParser α) : ByteArrayParser α := do
+def wrapped (tag : String) (p : Parser α) : Parser α := do
   expectS s!"<{tag}>"
   let s ← p
   expectS s!"</{tag}>"
   return s
 
-def wrappedArray (tag : String) (num : Nat) (p : ByteArrayParser α) : ByteArrayParser (Array α) := do
+def wrappedArray (tag : String) (num : Nat) (p : Parser α) : Parser (Array α) := do
   wrapped tag (readArray num p)
 
-def wrappedArrayString (tag : String) (num length : Nat) (f : String → String := (·.replace "\x00" "")) : ByteArrayParser (Array String) := do
+def wrappedArrayString (tag : String) (num length : Nat) (f : String → String := (·.replace "\x00" "")) : Parser (Array String) := do
   wrappedArray tag num s
 where
   s := do
@@ -23,7 +22,7 @@ where
     return f s
 
 @[inline]
-partial def manyCore (p : ByteArrayParser α) (acc : Array α) : ByteArrayParser (Array α) := do
+partial def manyCore (p : Parser α) (acc : Array α) : Parser (Array α) := do
   try
     let res ← p
     manyCore p (acc.push res)
@@ -31,9 +30,9 @@ partial def manyCore (p : ByteArrayParser α) (acc : Array α) : ByteArrayParser
     return acc
 
 @[inline]
-def many (p : ByteArrayParser α) : ByteArrayParser $ Array α := manyCore p #[]
+def many (p : Parser α) : Parser $ Array α := manyCore p #[]
 
-partial def readString' : ByteArrayParser String := do
+partial def readString' : Parser String := do
   let mut arr := ByteArray.empty
   repeat do
     let s ← peek
@@ -42,7 +41,7 @@ partial def readString' : ByteArrayParser String := do
     arr := arr.push s
   return arr |> String.fromUTF8Unchecked
 
-def release : ByteArrayParser Release := do
+def release : Parser Release := do
   match ←readString 3 with
   | "113" => return .«113»
   | "114" => return .«114»
@@ -50,45 +49,64 @@ def release : ByteArrayParser Release := do
   | "117" => return .«117»
   | "118" => return .«118»
   | "119" => return .«119»
-  | _     => error "invalid <release> field"
+  | _     => fail "invalid <release> field"
 
-def byteorder : ByteArrayParser Byteorder := do
+def byteorder : Parser Byteorder := do
   match ←readString 3 with
   | "LSF" => return .lsf
   | "MSF" => return .msf
-  | _      => error "invalid <byteorder> field"
+  | _      => fail "invalid <byteorder> field"
 
-def read16 : Byteorder → ByteArrayParser UInt16
+def read16 : Byteorder → Parser UInt16
 | .lsf => read16LE
 | .msf => read16BE
 
-def read32 : Byteorder → ByteArrayParser UInt32
+def read32 : Byteorder → Parser UInt32
 | .lsf => read32LE
 | .msf => read32BE
 
-def read64 : Byteorder → ByteArrayParser UInt64
+def read48 (bo : Byteorder) : Parser UInt64 := do
+  let a ← read8
+  let b ← read8
+  let c ← read8
+  let d ← read8
+  let e ← read8
+  let f ← read8 
+  return match bo with
+  | .lsf => a.toUInt64 ||| (b.toUInt64 <<< 8) ||| (c.toUInt64 <<< 16) ||| (d.toUInt64 <<< 24) ||| (e.toUInt64 <<< 32) ||| (f.toUInt64 <<< 40)
+  | .msf => f.toUInt64 ||| (e.toUInt64 <<< 8) ||| (d.toUInt64 <<< 16) ||| (c.toUInt64 <<< 24) ||| (b.toUInt64 <<< 32) ||| (a.toUInt64 <<< 40)
+
+def read64 : Byteorder → Parser UInt64
 | .lsf => read64LE
 | .msf => read64BE
 
-def k (r : Release) (e : Byteorder) : ByteArrayParser (typeK r) := by
+def readFloat : Byteorder → Parser Float
+| .lsf => readFloatLE
+| .msf => readFloatBE
+
+def readDouble : Byteorder → Parser Float
+| .lsf => readDoubleLE
+| .msf => readDoubleBE
+
+def k (r : Release) (e : Byteorder) : Parser (typeK r) := by
   cases r <;> simp [typeK]
   repeat exact read16 e
   exact read32 e
 
 def n (e : Byteorder) := read64 e
 
-def label (e : Byteorder) : ByteArrayParser String := do
+def label (e : Byteorder) : Parser String := do
   let length ← read16 e
   readString length.toNat
 
-def timestamp? : ByteArrayParser (Option String) := do
+def timestamp? : Parser (Option String) := do
   let length ← read8
   match length with
   |  0 => return none
   | 17 => return (←readString 17)
-  |  _ => error "length of timestamp must be 0 or 17"
+  |  _ => fail "length of timestamp must be 0 or 17"
 
-def header : ByteArrayParser Header := wrapped "header" do
+def header : Parser Header := wrapped "header" do
   let r ← wrapped "release" release
   let e ← wrapped "byteorder" byteorder
   let k ← wrapped "K" (k r e)
@@ -97,15 +115,15 @@ def header : ByteArrayParser Header := wrapped "header" do
   let timestamp? ← wrapped "timestamp" timestamp?
   return ⟨r, e, k, n, label, timestamp?⟩
 
-def map (e : Byteorder) : ByteArrayParser Map := do
+def map (e : Byteorder) : Parser Map := do
   wrappedArray "map" 14 (read64 e)
 
-def variableTypes (k : typeK r) (e : Byteorder) : ByteArrayParser VariableTypes := do
+def variableTypes (k : typeK r) (e : Byteorder) : Parser VariableTypes := do
   expectS "<variable_types>"
   let mut arr := #[]
   for x in ←readArray k.toNat (read16 e) do
     match x with
-    | 32768 => arr := arr.push .strL
+    | 32768 => arr := arr.push .strLIndex
     | 65526 => arr := arr.push .double
     | 65527 => arr := arr.push .float
     | 65528 => arr := arr.push .long
@@ -116,65 +134,108 @@ def variableTypes (k : typeK r) (e : Byteorder) : ByteArrayParser VariableTypes 
       if h : x' < 2045 then
         arr := arr.push <| .str ⟨x', h⟩
       else
-        throw (←error "variable type out of range")
+        throw (←fail "variable type out of range")
   expectS "</variable_types>"
   return arr
 
-def varnames (k : typeK r) : ByteArrayParser VarNames :=
+def varnames (k : typeK r) : Parser VarNames :=
   wrappedArrayString "varnames" k.toNat 129
 
-def sortlist (k : typeK r) (e : Byteorder) : ByteArrayParser SortList := do
+def sortlist (k : typeK r) (e : Byteorder) : Parser SortList := do
   wrappedArray "sortlist" (k.toNat + 1) (read16 e)
 
-def formats (k : typeK r) : ByteArrayParser Formats :=
+def formats (k : typeK r) : Parser Formats :=
   wrappedArrayString "formats" k.toNat 57
 
-def valueLabelNames (k : typeK r) : ByteArrayParser ValueLabelNames :=
+def valueLabelNames (k : typeK r) : Parser ValueLabelNames :=
   wrappedArrayString "value_label_names" k.toNat 129
 
-def variableLabels (k : typeK r) : ByteArrayParser VariableLabels := 
+def variableLabels (k : typeK r) : Parser VariableLabels := 
   wrappedArrayString "variable_labels" k.toNat 321 λ s => if s.startsWith "\x00" then "" else s.replace "\x00" ""
 
-def characteristic (e : Byteorder) : ByteArrayParser Characteristic := wrapped "ch" do
-  let _length ← read32 e
+def characteristic (e : Byteorder) : Parser Characteristic := wrapped "ch" do
+  let length ← read32 e
   let varname ← readString 129
   let charname ← readString 129
-  let contents ← many readString'
+  let contents ← readString (length.toNat - 258)
   return ⟨varname, charname, contents⟩
 
-def characteristics (e : Byteorder) : ByteArrayParser Characteristics := wrapped "characteristics" (many (characteristic e))
+def characteristics (e : Byteorder) : Parser Characteristics := wrapped "characteristics" (many (characteristic e))
 
-def observation (e : Byteorder) (k : typeK r) (ty : VariableType) : ByteArrayParser Observation := do
-  let p : ByteArrayParser (ty.toLeanType) := match ty with
-  | .str n => readString n.val
-  | .strL => sorry
-  | .double => read32 e |>.map uint32ToDouble
-  | .float => read16 e |>.map uint16ToFloat
-  | .long => read32 e
-  | .int => read16 e
-  | .byte => read8
-  sorry
+def readStrlIndex (e : Byteorder) : Parser (UInt32 × UInt64) := do
+  let a ← read16 e <&> UInt16.toUInt32
+  let b ← read48 e
+  return (a, b)
 
-def data (e : Byteorder) (k : typeK r) (varTypes : VariableTypes) : ByteArrayParser Data := wrapped "data" do
-  let mut obs := #[]
-  for ty in varTypes do
-    obs := obs.push (←observation k ty)
-  return obs
+def value (e : Byteorder) (ty : VariableType) : Parser Value :=
+  match ty with
+  | .str n => readString n.val <&> Value.str n
+  | .strLIndex => readStrlIndex e <&> Value.strLIndex
+  | .double => readDouble e <&> Value.double
+  | .float => readFloat e <&> Value.float
+  | .long => read32 e <&> Value.long
+  | .int => read16 e <&> Value.int
+  | .byte => read8 <&> Value.byte
 
-def dta : ByteArrayParser Dta := do
+def observation (e : Byteorder) (tys : VariableTypes) : Parser Observation := do
+  let mut arr := #[]
+  for ty in tys do
+    let v ← value e ty
+    arr := arr.push v
+  return arr
+
+def data (e : Byteorder) (n : UInt64) (tys : VariableTypes) : Parser Data :=
+  wrappedArray "data" n.toNat (observation e tys)
+
+def gso (e : Byteorder) : Parser GSO := do
+  expectS "GSO" 
+  let v ← read32 e
+  let o ← read64 e
+  let t ← read8
+  let len ← read32 e
+  match t with
+  | 129 => 
+    let content ← readString len.toNat
+    return ⟨v, o, true, len, content⟩
+  | 130 => 
+    let content ← readString'
+    return ⟨v, o, true, len, content⟩
+  | _ => throw (←fail s!"t must be 129 (binary) or 130 (ascii), but got {t}")
+
+def strLs (e : Byteorder) : Parser StrLs :=
+  wrapped "strls" <| many <| gso e
+
+def dta : Parser Dta := do
   expectS "<stata_dta>"
   let header ← header
-  let {k, byteorder := e, ..} := header
+  let {k, n, byteorder := e, ..} := header
   let map ← map e
   let varTypes ← variableTypes k e
   let varnames ← varnames k
+  dbg_trace "varnames"
+  dbg_trace repr varnames
   let sortlist ← sortlist k e
+  dbg_trace "sortlist"
+  dbg_trace sortlist
   let formats ← formats k
+  dbg_trace "format"
+  dbg_trace formats
   let valueLabelNames ← valueLabelNames k
+  dbg_trace "valueLabe"
+  dbg_trace valueLabelNames
   let variableLabels ← variableLabels k
+  dbg_trace "varLabel"
+  dbg_trace variableLabels
   let characteristics ← characteristics e
-  let data ← data e k varTypes
-  -- expectS "</stata_dta>"
-  return ⟨header, map, varTypes, varnames, sortlist, formats, valueLabelNames, variableLabels, characteristics, data⟩
+  dbg_trace "charac"
+  dbg_trace repr characteristics
+  let data ← data e n varTypes
+  dbg_trace "data"
+  dbg_trace repr data
+  let strLs ← strLs e
+  dbg_trace "strls"
+  dbg_trace repr strLs
+  expectS "</stata_dta>"
+  return ⟨header, map, varTypes, varnames, sortlist, formats, valueLabelNames, variableLabels, characteristics, data, strLs⟩
 
 end Dta
