git/xubaiw/Dta.lean/lakefile.lean
@@ -4,7 +4,7 @@ open Lake DSL
 package dta
 
 require parsec from
-  git "https://github.com/xubaiw/Parsec.lean"@"b6e8721c36bde18bca6a81e7b40d966b401cb329"
+  git "https://github.com/xubaiw/Parsec.lean"@"main"
 
 lean_lib Dta
 
